Add loop and procedure call in com. Add the required proof (a final Lemma on Hoare Triple remaind not verifiied)

Hoare_Triple.v
@@ -14,226 +14,349 @@ Definition hoare_triple (P Q: assertion) (c : com) (ps : Psi.psi) : Prop :=
 (* Some facts about Hoare Triples *)
 
 Lemma seq_hoare_triple :
-forall p1 p2 ps (P Q R: assertion),
-hoare_triple P R p1 ps ->
-hoare_triple R Q p2 ps ->
-hoare_triple P Q (CSeq p1 p2) ps.
+  forall p1 p2 ps (P Q R: assertion),
+    hoare_triple P R p1 ps ->
+    hoare_triple R Q p2 ps ->
+    hoare_triple P Q (CSeq p1 p2) ps.
 Proof.
-unfold hoare_triple.
-intros p1 p2 ps P Q R H1 H2 s s' Pre H12. inversion H12; subst.
-eapply H2. eapply H1. apply Pre. apply H3. apply H7.
+  unfold hoare_triple.
+  intros p1 p2 ps P Q R H1 H2 s s' Pre H12. inversion H12; subst.
+  eapply H2. eapply H1. apply Pre. apply H3. apply H7.
 Qed.
 
 Lemma if_hoare_triple :
-forall p1 p2 b ps (P Q: assertion),
-hoare_triple (fun s => P s /\ beval s b = true) Q p1 ps ->
-hoare_triple (fun s => P s /\ beval s b = false) Q p2 ps ->
-hoare_triple P Q (CIf b p1 p2) ps.
+  forall p1 p2 b ps (P Q: assertion),
+    hoare_triple (fun s => P s /\ beval s b = true) Q p1 ps ->
+    hoare_triple (fun s => P s /\ beval s b = false) Q p2 ps ->
+    hoare_triple P Q (CIf b p1 p2) ps.
 Proof.
-intros p1 p2 b ps P Q HTrue HFalse s s' HP HE.
-inversion HE;subst. 
-- unfold hoare_triple in HTrue.
-  eapply HTrue.
-  + split. 
+  intros p1 p2 b ps P Q HTrue HFalse s s' HP HE.
+  inversion HE;subst. 
+  - unfold hoare_triple in HTrue.
+    eapply HTrue.
+    + split. 
       * apply HP. 
       * assumption.
-  + apply H6.
-- unfold hoare_triple in HFalse.
-  eapply HFalse.
-  + split. 
+    + apply H6.
+  - unfold hoare_triple in HFalse.
+    eapply HFalse.
+    + split. 
       * apply HP. 
       * assumption.
-  + apply H6.
+    + apply H6.
 Qed.
 
 Lemma consequence_hoare_pre :
-forall p ps (P P' Q: assertion),
-hoare_triple P' Q p ps ->
-(forall s, P s -> P' s)->
-hoare_triple P Q p ps.
+  forall p ps (P P' Q: assertion),
+    hoare_triple P' Q p ps ->
+    (forall s, P s -> P' s)->
+    hoare_triple P Q p ps.
 Proof.
-unfold hoare_triple.
-intros.
-eapply H.
-apply H0.
-apply H1.
-apply H2.
+  unfold hoare_triple.
+  intros.
+  eapply H.
+  apply H0.
+  apply H1.
+  apply H2.
 Qed.
 
 Lemma consequence_hoare_post :
-forall p ps (P Q Q': assertion),
-hoare_triple P Q' p ps ->
-(forall s, Q' s -> Q s)->
-hoare_triple P Q p ps.
+  forall p ps (P Q Q': assertion),
+    hoare_triple P Q' p ps ->
+    (forall s, Q' s -> Q s)->
+    hoare_triple P Q p ps.
 Proof.
-unfold hoare_triple.
-intros.
-apply H0.
-eapply H.
-apply H1.
-apply H2.
+  unfold hoare_triple.
+  intros.
+  apply H0.
+  eapply H.
+  apply H1.
+  apply H2.
 Qed.
+
+Lemma while_hoare_triple : 
+  forall P b c ps,
+    hoare_triple (fun s => P s /\ beval s b = true) (P) c ps ->
+    hoare_triple (P) (fun s => P s /\ beval s b = false) (CWhile b c P) ps.
+Proof.
+  intros P b c ps Hhoare st st' HP Heval.
+  remember (CWhile b c P) as original_command eqn:Horig.
+  induction Heval.
+  * inversion Horig.
+  * inversion Horig.
+  * inversion Horig.
+  * inversion Horig.
+  * inversion Horig.
+  * inversion Horig.
+  * inversion Horig;subst. eauto.
+  * inversion Horig;subst.
+    eauto.
+  * inversion Horig.
+Qed.
+
+Lemma proc_hoare_triple : 
+  forall P Q f ps,
+    hoare_triple P Q (fst (ps f)) ps ->
+    hoare_triple P Q (CCall f) ps.
+Proof.
+  intros P Q f ps Hhoare st st' HP Heval.
+  unfold hoare_triple in Hhoare.
+  eapply Hhoare.
+  apply HP.
+  inversion Heval;subst.
+  apply H0.
+Qed.
+
+Definition hoare_triple_proc (ps : Psi.psi) : Prop :=
+  forall p , hoare_triple (get_pre (snd (ps p))) (get_post (snd (ps p))) (CCall p) ps.
+
+Definition hoare_triple_body (ps : Psi.psi) : Prop :=
+  forall p , hoare_triple (get_pre (snd (ps p))) (get_post (snd (ps p))) (fst (ps p)) ps.
+
+(*to be verified*)
+Axiom recursion_hoare_triple :
+  forall P Q p ps,
+    (hoare_triple_proc ps -> hoare_triple P Q p ps) ->
+    (hoare_triple_proc ps -> hoare_triple_body ps) ->
+    hoare_triple P Q p ps.
 
 (* Proof that one can use a verification condition generator to proof Hoare Triples *)
 
 Lemma correct :
-forall p ps,
-forall (P Q: assertion),
-(forall m, P m -> tc' p m ps) ->
-(forall m, P m -> tc p m ps Q) ->
-hoare_triple P Q p ps.
+  forall p ps,
+  forall (P Q: assertion),
+    (forall m, P m -> tc' p m ps) ->
+    (forall m, P m -> tc p m ps Q) ->
+    (hoare_triple_proc ps -> hoare_triple P Q p ps).
 Proof.
-intros p ps.
-induction p.
-* unfold hoare_triple. intros. eapply H0. apply H1. inversion H2;subst. reflexivity.
-* unfold hoare_triple. intros. eapply H0. apply H1. inversion H2;subst. reflexivity.
-* unfold hoare_triple. intros. eapply H0. apply H1. 
-  apply H. apply H1. inversion H2;subst. reflexivity. 
-* intros. eapply seq_hoare_triple.
+  intros p ps. 
+  induction p.
+  * unfold hoare_triple. intros. eapply H0. apply H2. inversion H3;subst. reflexivity.
+  * unfold hoare_triple. intros. eapply H0. apply H2. inversion H3;subst. reflexivity.
+  * unfold hoare_triple. intros. eapply H0. apply H2. 
+    apply H. apply H2. inversion H3;subst. reflexivity. 
+  * intros P Q Htc' Htc Hproc. eapply seq_hoare_triple.
   + apply IHp1.
-    - apply H.
-    - simpl in H0, H.
-     intros.
-     specialize (H m H1).
-     destruct H.
-     specialize (H0 m H1). 
-     specialize 
-     (tc_split p1 ps m (fun m' : sigma => tc' p2 m' ps) (fun m' : sigma => tc p2 m' ps Q)).
-     intros.
-     apply H3. assumption. assumption.
-  + apply IHp2.
-    - intros. destruct H1. assumption.
-    - intros. destruct H1. assumption.
-* intros. apply if_hoare_triple.
-  + apply IHp1.
-    - intros. apply H. apply H1. apply H1.
-    - intros. simpl in H. destruct H1. specialize (H0 m H1). destruct H0.
-      apply H0. apply bexp_eval_true. assumption.
-  + apply IHp2.
-    - intros. apply H. apply H1. destruct H1. apply bexp_eval_false in H2. apply H2.
-    - intros. simpl in H. destruct H1. specialize (H0 m H1). destruct H0.
-      apply H3. apply bexp_eval_false. assumption.
- Qed.
+  - apply Htc'.
+  - simpl in Htc', Htc.
+    intros.
+    specialize (Htc' m H).
+    destruct Htc'.
+    specialize (Htc m H). 
+    specialize 
+      (tc_split p1 ps m (fun m' : sigma => tc' p2 m' ps) (fun m' : sigma => tc p2 m' ps Q)).
+    intros.
+    apply H2. assumption. assumption.
+  - assumption.
+    + apply IHp2.
+  - intros. destruct H. assumption.
+  - intros. destruct H. assumption.
+  - assumption.
+    * intros P Q Htc' Htc Hproc. apply if_hoare_triple.
+    + apply IHp1.
+  - intros. apply Htc'. apply H. apply H.
+  - intros. simpl in Htc. destruct H. specialize (Htc m H). destruct Htc.
+    apply H1. apply bexp_eval_true. assumption.
+  - assumption.
+    + apply IHp2.
+  - intros. apply Htc'. apply H. destruct H. apply bexp_eval_false in H0. apply H0.
+  - intros. simpl in H. destruct H. specialize (Htc m H). destruct Htc.
+    apply H2. apply bexp_eval_false. assumption.
+  - assumption.
+    * intros  P Q Htc' Htc.
+      specialize (IHp (fun s => inv s /\ beval s b = true) inv).
+      intros Hproc s s' Pre.
+      apply (consequence_hoare_post _ _ P _ (fun s : sigma => inv s /\ beval s b = false)).
+    + apply (consequence_hoare_pre _ _ _ inv).  
+  - apply while_hoare_triple.
+    specialize (Htc s Pre).
+    specialize (Htc' s Pre).
+    simpl in Htc, Htc'.
+    destruct Htc'.
+    destruct H0. 
+    apply IHp.
+    ** intros.
+       apply H0.
+       destruct H2.
+       apply bexp_eval_true in H3.
+       assumption.
+    ** intros.
+       apply H1.
+       apply H2.
+    ** assumption.
+  - intros.
+    specialize (Htc' s0 H).
+    apply Htc'.
+    + intros.
+      specialize (Htc s Pre).
+      apply Htc.
+      specialize (Htc' s Pre).
+      apply Htc'.
+      apply H.
+      apply H.
+    + assumption.
+      * intros P Q Htc' Htc Hproc s s' Pre.
+        apply (consequence_hoare_post _ _ P _ (get_post (snd (ps f)))).
+    + apply (consequence_hoare_pre _ _ _ (get_pre (snd (ps f)))).
+  - apply Hproc.
+  - apply Htc'.
+    + eapply Htc.
+      apply Pre.
+      apply Htc'.
+      assumption.
+    + assumption.
+Qed.
+
+Lemma correct_proc :
+  forall ps,
+    tc_p ps ->
+    (hoare_triple_proc ps -> hoare_triple_body ps).
+Proof.
+  intros ps Htc Hproc.
+  unfold hoare_triple_body.
+  intros.
+  apply correct.
+  * apply Htc.
+  * apply Htc.
+  * assumption.
+Qed.
 
 (* Examples of proofs of Hoare Triples *)
 
 Example Hoare1 : hoare_triple (fun m => m EAX = 1) (fun m' => m' EAX = 3) plus2 Psi.empty_psi.
 Proof.
-apply correct.
-+ simpl;intros. auto.
-+ simpl;intros.
-  rewrite H0.
-  rewrite H.
-  simpl.
-  apply set'def.
-  reflexivity.
+  apply recursion_hoare_triple.
+  * apply correct.
+  + simpl;intros. auto.
+  + simpl;intros.
+    rewrite H0.
+    rewrite H.
+    simpl.
+    apply set'def.
+    reflexivity.
+    * apply correct_proc.
+      apply tc_p_empty_psi.
 Qed.
 
 Definition plus3 : com := CSeq (CAss EAX (APlus (AId EAX) (ANum 2)))
-                                (CAss EAX (APlus (AId EAX) (ANum 2))).
+                               (CAss EAX (APlus (AId EAX) (ANum 2))).
 
 Example Haore2 : hoare_triple (fun m => m EAX = 1) (fun m' => m' EAX = 5) plus3 Psi.empty_psi.
 Proof.
-apply correct.
-+ simpl;intros. auto.
-+ simpl;intros.
-  rewrite H1.
-  rewrite H0.
-  rewrite H.
-  simpl.
-  apply set'def.
-  reflexivity.
+  apply recursion_hoare_triple.
+  * apply correct.
+  + simpl;intros. auto.
+  + simpl;intros.
+    rewrite H1.
+    rewrite H0.
+    rewrite H.
+    simpl.
+    apply set'def.
+    reflexivity.
+    * apply correct_proc.
+      apply tc_p_empty_psi.
 Qed.
 
 Definition if2 : com := CIf (BEq (AId EAX) (ANum 4)) plus2 plus2.
 
 Example Hoare3 : hoare_triple (fun m => m EAX = 1) (fun m' => m' EAX = 3) if2 Psi.empty_psi .
 Proof.
-apply correct.
-+ simpl; intros.
-  auto.
-+ simpl;intros.
-  destruct (beval m (BEq (AId EAX) (ANum 4))) eqn:Hcond.
-  * split;intros.
-    - rewrite H1.
-      rewrite H.
-      apply set'def.
-      reflexivity.
-    - apply bexp_eval_true in Hcond.
-      contradiction H0.
-   * split;intros.
-    - apply bexp_eval_false in Hcond.
-      contradiction H0.
-    - rewrite H1.
-      rewrite H.
-      apply set'def.
-      reflexivity.
+  apply recursion_hoare_triple.
+  * apply correct.
+  + simpl; intros. auto.
+  + simpl;intros.
+    destruct (beval m (BEq (AId EAX) (ANum 4))) eqn:Hcond.
+  - split;intros.
+    ** rewrite H1.
+       rewrite H.
+       apply set'def.
+       reflexivity.
+    ** apply bexp_eval_true in Hcond.
+       contradiction H0.
+  - split;intros.
+    ** apply bexp_eval_false in Hcond.
+       contradiction H0.
+    ** rewrite H1.
+       rewrite H.
+       apply set'def.
+       reflexivity.
+    * apply correct_proc.
+      apply tc_p_empty_psi.
 Qed.
 
 Definition if3 : com := CSeq (CAss EAX (APlus (AId EAX) (ANum 2)))
-                            (CSeq (CIf (BEq (AId EAX) (ANum 4)) plus2 plus2) plus2).
+                             (CSeq (CIf (BEq (AId EAX) (ANum 4)) plus2 plus2) plus2).
 
 Example Hoare4 : hoare_triple (fun m => m EAX = 1) (fun m' => m' EAX = 7) if3 Psi.empty_psi.
 Proof.
-apply correct.
-+ simpl;intros. auto.
-+ simpl;intros.
-  destruct (beval m' (BEq (AId EAX) (ANum 4))) eqn:Hcond.
-  * split;intros.
-    - rewrite H3.
-      rewrite H2.
-      rewrite H0.
-      rewrite H.
-      apply set'def.
-      reflexivity.
-    - apply bexp_eval_true in Hcond.
-      contradiction H1.
-  * split;intros.
-    - apply bexp_eval_false in Hcond.
-      contradiction H1.
-    - rewrite H3.
-      rewrite H2.
-      rewrite H0.
-      rewrite H.
-      apply set'def.
-      reflexivity.
+  apply recursion_hoare_triple.
+  * apply correct.
+  + simpl;intros. auto.
+  + simpl;intros.
+    destruct (beval m' (BEq (AId EAX) (ANum 4))) eqn:Hcond.
+  - split;intros.
+    ** rewrite H3.
+       rewrite H2.
+       rewrite H0.
+       rewrite H.
+       apply set'def.
+       reflexivity.
+    ** apply bexp_eval_true in Hcond.
+       contradiction H1.
+  - split;intros.
+    ** apply bexp_eval_false in Hcond.
+       contradiction H1.
+    ** rewrite H3.
+       rewrite H2.
+       rewrite H0.
+       rewrite H.
+       apply set'def.
+       reflexivity.
+    * apply correct_proc.
+      apply tc_p_empty_psi.
 Qed.
 
 Definition assert3 : com := CSeq (CAssert (fun m => m EAX = 2))
-                          (CAssert (fun m => m EAX = 2)).
-                          
+                                 (CAssert (fun m => m EAX = 2)).
+
 Example Hoare6 : hoare_triple (fun m => m EAX = 2) (fun _ => True) assert3 Psi.empty_psi.
 Proof.
-apply correct.
-+ simpl;intros.
-  split.
-   * assumption.
-   * intros.
-      rewrite <- H1.
-      assumption.
-+ simpl; intros. auto.
+  apply recursion_hoare_triple.
+  * apply correct.
+  + simpl;intros.
+    split.
+  - assumption.
+  - intros.
+    rewrite <- H1.
+    assumption.
+    + simpl; intros. auto.
+      * apply correct_proc.
+        apply tc_p_empty_psi.
 Qed.
 
 Definition if4 : com := CIf (BEq (AId EAX) (ANum 2)) (CAssert (fun m => m EAX = 2)) CSkip.
 
 Example Hoare7 : hoare_triple (fun m => m EAX = 2) (fun m' => m' EAX = 2) if4 Psi.empty_psi.
 Proof.
-apply correct.
-+ simpl;intros. 
-  split.
-    * intros.
-      assumption.
-    * auto.
-+ simpl;intros.
-  destruct (beval m (BEq (AId EAX) (ANum 2))) eqn:Hcond.
-  * split;intros.
-    - rewrite <- H2.
-      assumption.
-    - apply bexp_eval_true in Hcond.
-      contradiction H0.
-  * split;intros.
-    - apply bexp_eval_false in Hcond.
-      contradiction H0.
-    - rewrite <- H1.
-      assumption.
+  apply recursion_hoare_triple.
+  * apply correct.
+  + simpl;intros. 
+    split.
+  - intros.
+    assumption.
+  - auto.
+    + simpl;intros.
+      destruct (beval m (BEq (AId EAX) (ANum 2))) eqn:Hcond.
+  - split;intros.
+    ** rewrite <- H2.
+       assumption.
+    ** apply bexp_eval_true in Hcond.
+       contradiction H0.
+  - split;intros.
+    ** apply bexp_eval_false in Hcond.
+       contradiction H0.
+    ** rewrite <- H1.
+       assumption.
+    * apply correct_proc.
+      apply tc_p_empty_psi.
 Qed.
